@WIP

NS/Misc.v
@@ -5,6 +5,7 @@ Require Import Coq.Strings.String.
 Require Import Coq.Arith.PeanoNat.
 Require Import Coq.Arith.EqNat.
 Require Import Coq.Bool.Bool.
+Require Import Coq.Logic.FunctionalExtensionality.
 Require Import Coq.Logic.Eqdep.
 
 Notation "a <| b" := (a b) (at level 102, right associativity, only parsing).
@@ -147,6 +148,17 @@ match a with
     cons_opt (option_map ((fun z => (x_key, z)) << f x) (js_record_assoc x_key b)) (js_record_zip_with f xs b)
 end.
 
+Definition JsRecordHasKey {A: Set} (key: string): js_record A -> Prop :=
+  List.Exists (fun '(key', _) => key = key').
+
+Inductive JsRecordAdd {A: Set} (key: string) (x: A) (xs: js_record A) (xs': js_record A) :=
+| JSRecordAdd_ (add: List.Add (key, x) xs xs') (not_in : not (JsRecordHasKey key xs)).
+
+Inductive JsRecordNoDup {A: Set} : js_record A -> Prop :=
+| JsRecordNoDupNil : JsRecordNoDup nil
+| JsRecordNoDupCons : forall kx vx xs, JsRecordNoDup xs -> not (JsRecordHasKey kx xs) -> JsRecordNoDup ((kx, vx) :: xs)%list
+.
+
 Lemma nat_ind2: forall (P: nat -> nat -> Prop),
     P 0 0 ->
     (forall x, P x 0 -> P (S x) 0) ->
@@ -225,6 +237,40 @@ Ltac remove_existTs :=
   | H : existT (fun x0 : Set => x0) ?A ?a = existT (fun x1 : Set => x1) ?B ?b |- _ => apply eq_sigT_fst in H
   end.
 Ltac inv H := inversion H; remove_existTs; subst; clear H; try discriminate.
+Ltac if_some tac H := lazymatch H with | None => idtac | @None => idtac | Some ?H => tac H | ?H => idtac H; fail "must be None or Some" end.
+
+Ltac fix_js_record_existTs :=
+  repeat match goal with
+  | H : existT (fun x : Set => x) (js_record ?T) ?a =
+        existT (fun x : Set => x) (list (string * ?T)) ?b |- _ =>
+      unfold js_record in H; apply inj_pair2 in H; subst
+  | H : existT (fun x : Set => x) (list (string * ?T)) ?a =
+        existT (fun x : Set => x) (js_record ?T) ?b |- _ =>
+      unfold js_record in H; apply inj_pair2 in H; subst
+  end.
+
+Ltac clear_obvious :=
+  repeat lazymatch goal with
+  | H : ?T = ?T |- _ => clear H
+  | H : True |- _ => clear H
+  end.
+
+Ltac invert_eqs :=
+  repeat lazymatch goal with
+  | H : ?f ?a ?a0 ?a1 ?a2 ?a3 ?a4 ?a5 = ?f ?b ?b0 ?b1 ?b2 ?b3 ?b4 ?b5 |- _ => inv H
+  | H : ?f ?a ?a0 ?a1 ?a2 ?a3 ?a4 = ?f ?b ?b0 ?b1 ?b2 ?b3 ?b4 |- _ => inv H
+  | H : ?f ?a ?a0 ?a1 ?a2 ?a3 = ?f ?b ?b0 ?b1 ?b2 ?b3 |- _ => inv H
+  | H : ?f ?a ?a0 ?a1 ?a2 = ?f ?b ?b0 ?b1 ?b2 |- _ => inv H
+  | H : ?f ?a ?a0 ?a1 = ?f ?b ?b0 ?b1 |- _ => inv H
+  | H : ?f ?a ?a0 = ?f ?b ?b0 |- _ => inv H
+  | H : ?f ?a = ?f ?b |- _ => inv H
+  | H : ?a = nil |- _ => rewrite H in *; clear H
+  end.
+
+Ltac revert_with t :=
+  repeat lazymatch goal with
+  | H : context[t] |- _ => revert H
+  end.
 
 Ltac assert_specialize H :=
   let tH := type of H in
@@ -239,3 +285,169 @@ Ltac split_with H :=
 
 Ltac left_right_with H :=
   destruct H as [H | H]; [left | right].
+
+Lemma list_add_ind : forall {A: Type} (P: list A -> Prop),
+    P nil ->
+    (forall xs', (exists x xs, P xs /\ List.Add x xs xs') -> P xs') ->
+    forall xs, P xs.
+Proof.
+  intros A P P0 Pn xs; induction xs; [exact P0 |].
+  apply Pn; eexists; eexists; split; [exact IHxs |].
+  apply List.Add_head.
+Qed.
+
+Ltac rewrite_Forall_Exists_neg A key :=
+  replace (fun '(key', _) => key <> key') with (fun (x: string * A) => not ((fun '(key', _) => key = key') x)) in *;
+  try (apply functional_extensionality; destruct 0; reflexivity);
+  rewrite List.Forall_Exists_neg in *.
+
+Theorem JsRecordHasKey_dec: forall {A: Set} (key: string) (xs: js_record A),
+    JsRecordHasKey key xs \/ not (JsRecordHasKey key xs).
+Proof.
+  intros; induction xs.
+  - right; intros H; inversion H.
+  - destruct a; destruct (string_dec key s).
+    + left; subst; apply List.Exists_cons_hd; reflexivity.
+    + destruct IHxs; [left | right].
+      * apply List.Exists_cons_tl; exact H.
+      * intros H0; inversion H0; subst.
+        --  contradiction (n eq_refl).
+        --  contradiction (H H2).
+Qed.
+
+Theorem JsRecordHasKey_neg: forall {A: Set} (key: string) (xs: js_record A),
+    not (JsRecordHasKey key xs) <-> List.Forall (fun '(key', _) => key <> key') xs.
+Proof.
+  split; intros; rewrite_Forall_Exists_neg A key; exact H.
+Qed.
+
+Theorem JsRecordHasKey_alt: forall {A: Set} (key: string) (xs: js_record A),
+    JsRecordHasKey key xs <-> not (List.Forall (fun '(key', _) => key <> key') xs).
+Proof.
+  split; intros; rewrite_Forall_Exists_neg A key.
+  - intros H0; contradiction (H0 H).
+  - apply Decidable.not_not; unfold Decidable.decidable; [apply JsRecordHasKey_dec | exact H].
+Qed.
+
+Lemma JsRecordHasKey_neg_Add : forall {A: Set} (kx' : string) (xs': js_record A),
+  not (JsRecordHasKey kx' xs') ->
+  forall (kx: string) (vx: A) (xs: js_record A),
+  List.Add (kx, vx) xs xs' ->
+  kx' <> kx /\ not (JsRecordHasKey kx' xs).
+Proof.
+  intros A kx' xs'; induction xs'; intros; inv H0; rewrite JsRecordHasKey_neg in *; inv H.
+  - split; assumption.
+  - destruct a; subst; rename s into kx0; split.
+    + intros H; subst.
+      rewrite List.Forall_forall in H4;
+        pose (H := List.Add_in H3); pose (H0 := List.in_eq (kx, vx) l); rewrite <- H in H0; specialize (H4 _ H0); simpl in H4; contradiction (H4 eq_refl).
+    + apply List.Forall_cons; [exact H2 |]. rewrite <- JsRecordHasKey_neg; eapply proj2; eapply (IHxs' H4); exact H3.
+Qed.
+
+Lemma JsRecordHasKey_neg_Add0 : forall {A: Set} (kx' : string) (xs': js_record A),
+  not (JsRecordHasKey kx' xs') ->
+  forall (kx: string) (vx: A) (xs: js_record A),
+  List.Add (kx, vx) xs xs' ->
+  not (JsRecordHasKey kx' xs).
+Proof.
+  intros; eapply proj2; eapply JsRecordHasKey_neg_Add; [exact H | exact H0].
+Qed.
+
+Lemma JsRecordNoDup_alt0 : forall {A: Set} (xs': js_record A),
+  JsRecordNoDup xs' ->
+  forall (kx: string) (vx: A) (xs: js_record A),
+  List.Add (kx, vx) xs xs' ->
+  JsRecordNoDup xs.
+Proof.
+  intros A xs'; induction xs'; intros; inv H0; inv H; [exact H2 |];
+    apply JsRecordNoDupCons.
+  - apply (IHxs' H2 kx vx); exact H3.
+  - eapply (JsRecordHasKey_neg_Add0 H4); exact H3.
+Qed.
+
+Lemma JsRecordNoDup_alt1 : forall {A: Set} (xs': js_record A),
+  JsRecordNoDup xs' ->
+  forall (kx: string) (vx: A) (xs: js_record A),
+  List.Add (kx, vx) xs xs' ->
+  not (JsRecordHasKey kx xs).
+Proof.
+  intros A xs'; induction xs'; intros; inv H0; inv H; [exact H4 |];
+    rewrite JsRecordHasKey_neg; apply List.Forall_cons.
+  - intros H; subst;
+      rewrite JsRecordHasKey_neg, List.Forall_forall in H4;
+      pose (H := List.Add_in H3); pose (H0 := List.in_eq (kx0, vx) l); rewrite <- H in H0; specialize (H4 _ H0); simpl in H4; contradiction (H4 eq_refl).
+  - rewrite <- JsRecordHasKey_neg. eapply IHxs'; [exact H2 | exact H3].
+Qed.
+
+Lemma JsRecordNoDup_alt : forall {A: Set} (kx: string) (vx: A) (xs xs': js_record A),
+  JsRecordNoDup xs' ->
+  List.Add (kx, vx) xs xs' ->
+  JsRecordNoDup xs /\ not (JsRecordHasKey kx xs).
+Proof.
+  split; [eapply JsRecordNoDup_alt0 | eapply JsRecordNoDup_alt1]; [exact H | exact H0 | exact H | exact H0].
+Qed.
+
+Lemma js_record_destruct : forall {A: Set} (xs: js_record A),
+    xs = nil \/ forall kx vx, ~ JsRecordHasKey kx xs -> exists xs', JsRecordAdd kx vx xs xs'.
+Proof.
+  intros; induction xs; [left; reflexivity | right]. destruct a as [kx0 vx0]. destruct IHxs.
+  - subst. intros. destruct (string_dec kx0 kx).
+    + subst. contradict H. apply List.Exists_cons_hd. reflexivity.
+    + exists ((kx, vx) :: (kx0, vx0) :: nil)%list. split.
+      * apply List.Add_head.
+      * intros H0. inv H0; [contradiction (n eq_refl) | inv H2].
+  - intros. specialize (H kx vx). assert (~ JsRecordHasKey kx xs).
+      intros H1. contradict H0. apply List.Exists_cons_tl. unfold JsRecordHasKey in H1. exact H1.
+    specialize (H H1). destruct H as [xs' H]. exists ((kx0, vx0) :: xs')%list. split_with H.
+    + apply List.Add_cons. exact H.
+    + exact H0.
+Qed.
+
+Lemma js_record_ind : forall {A: Set} (P: js_record A -> Prop),
+    P nil ->
+    (forall xs', (exists kx vx xs, ~JsRecordHasKey kx xs -> P xs /\ JsRecordAdd kx vx xs xs') -> P xs') ->
+    forall xs, P xs.
+Proof.
+  intros A P P0 Pn xs.
+  induction xs using list_add_ind; intros; [exact P0 |]; destruct H as [[kx vx] [xs [H0 H1]]].
+  eapply Pn. do 3 eexists. intros. split; [exact H0 |]. split; [exact H1 | exact H].
+Qed.
+
+Lemma JsRecordAdd_HasKey : forall {A: Set} (kx: string) (vx: A) (xs xs': js_record A),
+    JsRecordAdd kx vx xs xs' -> JsRecordHasKey kx xs'.
+Proof.
+  intros. inv H. eapply List.Add_in in add. assert (List.In (kx, vx) ((kx, vx) :: xs)%list).
+    simpl. left. reflexivity.
+  rewrite <- add in H. clear add. rewrite JsRecordHasKey_alt, List.Forall_forall. intros H0. specialize (H0 (kx, vx) H). simpl in H0. contradiction (H0 eq_refl).
+Qed.
+
+Lemma js_record_ind2 : forall {A: Set} (P: js_record A -> js_record A -> Prop),
+    P nil nil ->
+    (forall xs', (exists kx vx xs, ~JsRecordHasKey kx xs -> P xs nil /\ JsRecordAdd kx vx xs xs') -> P xs' nil) ->
+    (forall ys', (exists ky vy ys, ~JsRecordHasKey ky ys -> P nil ys /\ JsRecordAdd ky vy ys ys') -> P nil ys') ->
+    (forall xs' ys', (exists kx vx ky vy xs ys, ~JsRecordHasKey kx xs -> ~JsRecordHasKey ky ys -> P xs ys /\ JsRecordAdd kx vx xs xs' /\ JsRecordAdd ky vy ys ys') -> P xs' ys') ->
+    forall xs ys, P xs ys.
+Proof.
+  intros A P P0 Px Py Pxy xs. induction xs; intros; induction ys.
+  - exact P0.
+  - destruct a as [ky vy]. apply Py. exists ky. exists vy. exists ys. split; [| split].
+    + exact IHys.
+    + apply List.Add_head.
+    + exact H.
+  - destruct a as [kx vx]. apply Px. exists kx. exists vx. exists xs. split; [| split].
+    + exact (IHxs nil).
+    + apply List.Add_head.
+    + exact H.
+  - destruct a as [kx vx]. destruct a0 as [ky vy]. apply Pxy. exists kx. exists vx. exists ky. exists vy. exists xs. exists ys. intros. split; [| split; split].
+    + exact (IHxs ys).
+    + apply List.Add_head.
+    + exact H.
+    + apply List.Add_head.
+    + exact H0.
+Qed.
+
+Ltac ind_js_record2 x y :=
+  revert x y;
+  match goal with
+  | [ |- forall x y, ?H ] => apply (js_record_ind2 (fun x y => H))
+  end.
